Changes in desugaring for proving binding instantiation.

LambdaS5/tests/es5/eval_nonstrict_var.in.js
@@ -1,0 +1,1 @@
+try { throw 1 } catch (x) { eval("var y = 2") }; y
