LambdaS5/coq/EjsFromJs.v
@@ -66,7 +66,7 @@ Fixpoint js_expr_to_ejs (e : J.expr) : E.expr :=
     | J.expr_assign e1 oo e2 => E.expr_assign (js_expr_to_ejs e1) oo (js_expr_to_ejs e2)
     | J.expr_new e es => E.expr_new (js_expr_to_ejs e) (List.map js_expr_to_ejs es)
     | J.expr_call e es => E.expr_app (js_expr_to_ejs e) (List.map js_expr_to_ejs es)
-    | J.expr_function onm xs (J.funcbody_intro p s) => E.expr_func onm xs (js_prog_to_ejs p) s
+    | J.expr_function onm xs (J.funcbody_intro p s) => E.expr_func onm (E.func_intro xs (js_prog_to_ejs p) s)
     | J.expr_object ps => 
         E.expr_object (List.map (fun (pp : J.propname * J.propbody) => let (pn, p) := pp in (JI.string_of_propname pn, js_prop_to_ejs p)) ps) 
     | J.expr_array oes => E.expr_array (List.map (fun oe => LibOption.map js_expr_to_ejs oe) oes)
@@ -74,8 +74,10 @@ Fixpoint js_expr_to_ejs (e : J.expr) : E.expr :=
 with js_prop_to_ejs p :=
     match p with
     | J.propbody_val e => E.property_data (js_expr_to_ejs e)
-    | J.propbody_get (J.funcbody_intro p s) => E.property_getter (E.expr_func None nil (js_prog_to_ejs p) s)
-    | J.propbody_set is (J.funcbody_intro p s) => E.property_setter (E.expr_func None is (js_prog_to_ejs p) s)
+    | J.propbody_get (J.funcbody_intro p s) => 
+        E.property_getter (E.expr_func None (E.func_intro nil (js_prog_to_ejs p) s))
+    | J.propbody_set is (J.funcbody_intro p s) => 
+        E.property_setter (E.expr_func None (E.func_intro is (js_prog_to_ejs p) s))
     end
 with js_stat_to_ejs (e : J.stat) : E.expr := 
     match e with
@@ -159,19 +161,41 @@ with js_switchclause_to_ejs c :=
 with js_element_to_ejs (e : J.element) : E.expr := 
     match e with
     | J.element_stat st => js_stat_to_ejs st
-    | J.element_func_decl s ps (J.funcbody_intro p s') => 
-(* TODO reconsider implementation strategy *)
-        E.expr_func_stmt s ps (js_prog_to_ejs p) s'
+    | J.element_func_decl s ps (J.funcbody_intro p s') => E.expr_empty
+    end
+with js_element_to_func (e : J.element) : list (E.id * E.func) :=
+    match e with
+    | J.element_stat st => nil
+    | J.element_func_decl s ps (J.funcbody_intro p s') => [(s, E.func_intro ps (js_prog_to_ejs p) s')]
     end
 with js_prog_to_ejs p : E.prog :=
-    let js_elements_to_ejs (es : list J.element) : E.expr :=
-        let filtmap_js_element_to_ejs p := fix f l :=
-            match l with nil => nil | e :: es => if p e then js_element_to_ejs e :: f es else f es end in
-        E.expr_seqs (filtmap_js_element_to_ejs is_element_func_decl es ++ 
-            filtmap_js_element_to_ejs is_element_stat es) in
     match p with
-    | J.prog_intro b sts => E.prog_intro b (JI.prog_vardecl p) (js_elements_to_ejs sts)
+    | J.prog_intro b sts => 
+        E.prog_intro b (concat (List.map js_element_to_func sts))
+            (JI.prog_vardecl p) (E.expr_seqs (List.map js_element_to_ejs sts))
     end.
+
+Definition js_funcdecl_to_func (fd : J.funcdecl) : E.id * E.func :=
+    match fd with
+    | J.funcdecl_intro s ps (J.funcbody_intro p s') => 
+        (s, E.func_intro ps (js_prog_to_ejs p) s')
+    end.
+
+Lemma js_element_to_func_lemma : forall el,
+    js_element_to_func el = map js_funcdecl_to_func (JI.element_funcdecl el).
+Proof.
+    introv.
+    destruct el as [?|? ? [? ?]]; simpl; rew_map; reflexivity.
+Qed.
+
+Lemma js_funcdecl_to_func_lemma : forall p,
+    E.prog_funcs (js_prog_to_ejs p) = map js_funcdecl_to_func (JI.prog_funcdecl p).
+Proof.
+    introv. 
+    destruct p. unfolds JI.prog_funcdecl. induction l; simpls; repeat (rew_map || rew_concat). 
+    + reflexivity.
+    + rewrite js_element_to_func_lemma. rewrite IHl. reflexivity.
+Qed.
 
 Require EjsToLjs.
 
